start saturated-arithmetic API for use in Montgomery (see discussion in #157)

src/Arithmetic/Saturated.v
@@ -404,26 +404,25 @@ Module Columns.
         autorewrite with uncps push_id push_basesystem_eval in *.
         rewrite eval_cons_to_nth by omega. nsatz.
     Qed.
-
+    
   End Columns.
 
   Section Wrappers.
-    Context (weight : nat->Z)
-            {add_get_carry: Z ->Z -> Z -> (Z * Z)}
-            {div modulo : Z -> Z -> Z}.
+    Context (weight : nat->Z).
 
-    Definition add_cps {n} (p q : Z^n) {T} (f : (Z*Z^n)->T) :=
+    Definition add_cps {n1 n2 n3} (p : Z^n1) (q : Z^n2)
+               {T} (f : (Z*Z^n3)->T) :=
       B.Positional.to_associational_cps weight p
         (fun P => B.Positional.to_associational_cps weight q
-        (fun Q => from_associational_cps weight n (P++Q)
-        (fun R => compact_cps (div:=div) (modulo:=modulo) (add_get_carry:=add_get_carry) weight R f))).
+        (fun Q => from_associational_cps weight n3 (P++Q)
+        (fun R => compact_cps (div:=div) (modulo:=modulo) (add_get_carry:=Z.add_get_carry_full) weight R f))).
 
     Definition sub_cps {n} (p q : Z^n) {T} (f : (Z*Z^n)->T) :=
       B.Positional.to_associational_cps weight p
         (fun P => B.Positional.negate_snd_cps weight q
         (fun nq => B.Positional.to_associational_cps weight nq
         (fun Q => from_associational_cps weight n (P++Q)
-        (fun R => compact_cps (div:=div) (modulo:=modulo) (add_get_carry:=add_get_carry) weight R f)))).
+        (fun R => compact_cps (div:=div) (modulo:=modulo) (add_get_carry:=Z.add_get_carry_full) weight R f)))).
 
     End Wrappers.
 End Columns.
@@ -452,15 +451,12 @@ Section Freeze.
             {weight_positive : forall i, weight i > 0}
             {weight_multiples : forall i, weight (S i) mod weight i = 0}
             {weight_divides : forall i : nat, weight (S i) / weight i > 0}
-            {div modulo : Z -> Z -> Z}
-            {div_correct : forall a b, div a b = a / b}
-            {modulo_correct : forall a b, modulo a b = a mod b}
     .
 
     Definition conditional_add_cps {n} mask cond (p q : Z^n)
                {T} (f:_->T) :=
       B.Positional.select_cps mask cond q
-                 (fun qq => Columns.add_cps (div:=div) (modulo:=modulo) (add_get_carry:=Z.add_get_carry_full) weight p qq f).
+                 (fun qq => Columns.add_cps (n3:=n) weight p qq f).
     Definition conditional_add {n} mask cond p q :=
       @conditional_add_cps n mask cond p q _ id.
     Lemma conditional_add_id {n} mask cond p q T f:
@@ -482,6 +478,7 @@ Section Freeze.
       repeat progress autounfold in *.
     pose proof Z.add_get_carry_full_mod.
     pose proof Z.add_get_carry_full_div.
+    pose proof div_correct. pose proof modulo_correct.
     autorewrite with uncps push_id push_basesystem_eval.
     break_match;
       match goal with
@@ -509,8 +506,7 @@ Section Freeze.
     the carry in step 3 was -1, so they cancel out.
    *)
   Definition freeze_cps {n} mask (m:Z^n) (p:Z^n) {T} (f : Z^n->T) :=
-    Columns.sub_cps (div:=div) (modulo:=modulo)
-                    (add_get_carry:=Z.add_get_carry_full) weight p m
+    Columns.sub_cps weight p m
       (fun carry_p => conditional_add_cps mask (fst carry_p) (snd carry_p) m
       (fun carry_r => f (snd carry_r)))
   .
@@ -569,6 +565,7 @@ Section Freeze.
     repeat progress autounfold.
     pose proof Z.add_get_carry_full_mod.
     pose proof Z.add_get_carry_full_div.
+    pose proof div_correct. pose proof modulo_correct.
     autorewrite with uncps push_id push_basesystem_eval.
 
     pose proof (weight_nonzero n).
@@ -588,6 +585,118 @@ Section Freeze.
       reflexivity. }
   Qed.
 End Freeze.
+
+Section API.
+  Context {weight : nat -> Z}
+          {weight_0 : weight 0%nat = 1}
+          {weight_nonzero : forall i, weight i <> 0}
+          {weight_positive : forall i, weight i > 0}
+          {weight_multiples : forall i, weight (S i) mod weight i = 0}
+          {weight_divides : forall i : nat, weight (S i) / weight i > 0}
+  .
+
+  Definition T : Type := list Z.
+
+  Definition length : T -> nat := @length Z.
+
+  Definition divmod (p : T) : T * Z :=
+    (List.tl p, List.hd 0 p).
+
+  (* TODO : scmul  (Z -> T -> T), using double-output multiply *)
+
+  Definition add (p q : T) : T * Z :=
+    let P := Tuple.from_list (Datatypes.length p) p (eq_refl _) in
+    let Q := Tuple.from_list (Datatypes.length q) q (eq_refl _) in
+    let n := max (Datatypes.length p) (Datatypes.length q) in
+    let carry_result := Columns.add_cps weight P Q id in
+    (to_list n (snd carry_result), fst carry_result).
+
+  Definition join (to_join : T * Z) : T :=
+    let p := fst to_join in
+    let P := Tuple.from_list (Datatypes.length p) p (eq_refl _) in
+    to_list _ (left_append (snd to_join) P).
+  
+  Section Proofs.
+    Definition eval (p : T) : Z :=
+      B.Positional.eval weight (Tuple.from_list (Datatypes.length p) p (eq_refl _)).
+
+    Lemma eval_add_nz p q :
+      max (Datatypes.length p) (Datatypes.length q) <> 0%nat ->
+      eval (fst (add p q)) = eval p + eval q - snd (add p q) * weight (Datatypes.length (fst (add p q))).
+    Proof.
+      intros.
+      pose proof Z.add_get_carry_full_div.
+      pose proof Z.add_get_carry_full_mod.
+      pose proof div_correct. pose proof modulo_correct.
+      repeat match goal with
+             | _ => progress (cbv [add eval]; repeat autounfold)
+             | _ => progress autorewrite with uncps push_id cancel_pair push_basesystem_eval
+             | _ => progress
+                      (rewrite <-!from_list_default_eq with (d:=0);
+                       erewrite !length_to_list, !from_list_default_eq,
+                       from_list_to_list)
+             | _ => rewrite Z.mul_div_eq' by auto using weight_nonzero;
+                      omega
+             end.
+      Unshelve. distr_length.
+    Qed.
+
+    Lemma eval_add_z p q :
+      max (Datatypes.length p) (Datatypes.length q) = 0%nat ->
+      eval (fst (add p q)) = eval p + eval q - snd (add p q) * weight (Datatypes.length (fst (add p q))).
+    Proof. destruct p, q; distr_length; reflexivity. Qed.
+
+    Lemma eval_add p q : 
+      eval (fst (add p q)) = eval p + eval q - snd (add p q) * weight (Datatypes.length (fst (add p q))).
+    Proof.
+      destruct (Nat.eq_dec (max (Datatypes.length p) (Datatypes.length q)) 0%nat); auto using eval_add_z, eval_add_nz.
+    Qed.
+    Hint Rewrite eval_add : push_basesystem_eval.
+    
+    Lemma eval_join to_join :
+      eval (join to_join) = eval (fst to_join) + snd to_join * weight (Datatypes.length (fst to_join)).
+    Proof.
+      repeat match goal with
+             | _ => progress (cbv [join eval]; repeat autounfold)
+             | _ => progress autorewrite with uncps push_id cancel_pair push_basesystem_eval
+             | _ => progress
+                      (rewrite <-!from_list_default_eq with (d:=0);
+                       erewrite !length_to_list, !from_list_default_eq,
+                       from_list_to_list)
+             | _ => rewrite B.Positional.eval_left_append; ring_simplify; omega
+             end.
+      Unshelve. distr_length.
+    Qed.
+    Hint Rewrite eval_join : push_basesystem_eval.
+
+    Lemma eval_join_add p q :
+      eval (join (add p q)) = eval p + eval q.
+    Proof. autorewrite with push_basesystem_eval; omega. Qed.
+
+    (* TODO : move to tuple *)
+    Lemma from_list_tl {A n} (ls : list A) H H':
+      from_list n (List.tl ls) H = tl (from_list (S n) ls H').
+    Proof.
+      induction ls; distr_length. simpl List.tl.
+      rewrite from_list_cons, tl_append, <-!(from_list_default_eq a ls).
+      reflexivity.
+    Qed.
+    
+    Lemma divmod_div p : eval (fst (divmod p)) = eval p / weight 1.
+    Proof.
+      repeat match goal with
+             | _ => progress (cbv [divmod eval]; repeat autounfold)
+             | _ => progress autorewrite with uncps push_id cancel_pair push_basesystem_eval
+             end.
+      erewrite from_list_tl.
+    Admitted.
+    
+    Lemma divmod_mod p : eval (fst (divmod p)) = eval p / weight 1.
+    Proof.
+    Admitted.
+      
+  End Proofs.
+End API.
 
 
 (*
